\section{Definitions of the evaluated relations}
\label{sec:examples_definitions}

Here are the definitions of the \mK relations we used for evaluation. Different queries to the same relation may require different orders in conjunctions.

\begin{enumerate}

\item Comparison of Peano numbers

\begin{minipage}{\linewidth}
Definition:

\begin{lstlisting}[basicstyle=\small]
   le$^o$ = fun x y ->
     (x === O) \/
     (fresh (x' y')
        (x === S(x')) /\
        (y === S(y')) /\
        (le$^o$ x' y')
     )
\end{lstlisting}
\end{minipage}

\begin{minipage}{\linewidth}
For queries:

\begin{itemize}
\item[-] \lstinline{le$^o$ $\overline{n}$ $\overline{m}$}

\item[-] \lstinline{le$^o$ $x^?$ $\overline{m}$}

\item[-] \lstinline{le$^o$ $\overline{n}$ $y^?$}
\end{itemize}
\end{minipage}


\item Sum of Peano numbers

\begin{minipage}{\linewidth}
Definition:

\begin{lstlisting}[basicstyle=\small]
   plus$^o$ = fun x y r ->
     ((x === O) /\ (y === r)) \/
     (fresh (x' r')
        (x === S(x')) /\
        (r === S(r')) /\
        (plus$^o$ x' y r')
     )
\end{lstlisting}
\end{minipage}

\begin{minipage}{\linewidth}
For queries:

\begin{itemize}
\item[-] \lstinline{plus$^o$ $\overline{n}$ $\overline{m}$ $r^?$}

\item[-] \lstinline{plus$^o$ $\overline{n}$ $y^?$ $\overline{k}$}

\item[-] \lstinline{plus$^o$ $x^?$ $y^?$ $\overline{k}$}
\end{itemize}
\end{minipage}


\item Product of Peano numbers

\begin{minipage}{\linewidth}
Definition \#1:

\begin{lstlisting}[basicstyle=\small]
   mult$^o$ = fun x y r ->
     ((x === O) /\ (r === O)) \/
     (fresh (x' r')
        (x === S(x')) /\
        (mult$^o$ x' y r') /\
        (plus$^o$ r' y r)
     )
\end{lstlisting}
\end{minipage}

\begin{minipage}{\linewidth}
For query:

\begin{itemize}
\item[-] \lstinline{mult$^o$ $\overline{n}$ $\overline{m}$ $r^?$}
\end{itemize}
\end{minipage}

\begin{minipage}{\linewidth}
Definition \#2:

\begin{lstlisting}[basicstyle=\small]
   mult$^o$ = fun x y r ->
     ((x === O) /\ (r === O)) \/
     (fresh (x' r')
        (x === S(x')) /\
        (plus$^o$ r' y r) /\
        (mult$^o$ x' y r')
     )
\end{lstlisting}
\end{minipage}

\begin{minipage}{\linewidth}
For queries:

\begin{itemize}
\item[-] \lstinline{mult$^o$ $x^?$ $\overline{m + 1}$ $\overline{k}$}

\item[-] \lstinline{mult$^o$ S($x^?$) S($y^?$) $\overline{k}$}
\end{itemize}
\end{minipage}


\item Length of a list

\begin{minipage}{\linewidth}
Definition \#1:

\begin{lstlisting}[basicstyle=\small]
   length$_d^o$ = fun a r ->
     ((a === Nil) /\ (x === O)) \/
     (fresh (h t r')
        (a === Cons(h, t)) /\
        (length$_d^o$ t r') /\
        (r === S(r'))
     )
\end{lstlisting}
\end{minipage}

\begin{minipage}{\linewidth}
For query:

\begin{itemize}
\item[-] \lstinline{length$_d^o$ $\overline{l}$ $r^?$}
\end{itemize}
\end{minipage}

\begin{minipage}{\linewidth}
Definition \#2:

\begin{lstlisting}[basicstyle=\small]
   length$^o$ = fun a r ->
     ((a === Nil) /\ (x === O)) \/
     (fresh (h t r')
        (a === Cons(h, t)) /\
        (r === S(r')) /\
        (length$^o$ t r')
     )
\end{lstlisting}
\end{minipage}

\begin{minipage}{\linewidth}
For queries:

\begin{itemize}
\item[-] \lstinline{length$^o$ $\overline{l}$ $r^?$}

\item[-] \lstinline{length$^o$ $a^?$ $\overline{n}$}
\end{itemize}
\end{minipage}


\item Incrementing all elements in a list

\begin{minipage}{\linewidth}
Definition:

\begin{lstlisting}[basicstyle=\small]
   incr_list$^o$ = fun a r ->
     ((a === Nil) /\ (r === Nil)) \/
     (fresh (h t tr)
        (a === Cons(h, t)) /\
        (r === Cons(S(h), tr)) /\
        (incr_list$^o$ t tr)
     )
\end{lstlisting}
\end{minipage}

\begin{minipage}{\linewidth}
For queries:

\begin{itemize}
\item[-] \lstinline{incr_list$^o$ $\overline{l}$ $r^?$}

\item[-] \lstinline{incr_list$^o$ $a^?$ $\overline{l}$}
\end{itemize}
\end{minipage}



\item Concatination of two lists

\begin{minipage}{\linewidth}
Definition:

\begin{lstlisting}[basicstyle=\small]
   append$^o$ = fun a b r ->
     ((a === Nil) /\ (b === r)) \/
     (fresh (h t tb)
        (a === Cons(h, t)) /\
        (r === Cons(h, tb)) /\
        (append$^o$ t b tb)
     )
\end{lstlisting}
\end{minipage}

\begin{minipage}{\linewidth}
For queries:

\begin{itemize}
\item[-] \lstinline{append$^o$ $\overline{l_1}$ $\overline{l_2}$ $r^?$}

\item[-] \lstinline{append$^o$ $a^?$ $b^?$ $\overline{l}$}
\end{itemize}
\end{minipage}


\item Inversion of a list

\begin{minipage}{\linewidth}
Definition \#1:

\begin{lstlisting}[basicstyle=\small]
   reverse$^o$ = fun a r ->
     ((a === Nil) /\ (r === Nil)) \/
     (fresh (h t tb)
        (a === Cons(h, t)) /\
        (reverse$^o$ t tr) /\
        (append$^o$ tr Cons(h, Nil) r)
     )
\end{lstlisting}
\end{minipage}

\begin{minipage}{\linewidth}
For query:

\begin{itemize}
\item[-] \lstinline{reverse$^o$ $\overline{l}$ $r^?$}
\end{itemize}
\end{minipage}
 
\begin{minipage}{\linewidth}
Definition \#2:

\begin{lstlisting}[basicstyle=\small]
   reverse$^o$ = fun a r ->
     ((a === Nil) /\ (r === Nil)) \/
     (fresh (h t tb)
        (a === Cons(h, t)) /\
        (append$^o$ tr Cons(h, Nil) r) /\
        (reverse$^o$ t tr)
     )
\end{lstlisting}
\end{minipage}

\begin{minipage}{\linewidth}
For query:

\begin{itemize}
\item[-] \lstinline{reverse$^o$ $a^?$ $\overline{l}$}
\end{itemize}
\end{minipage}

\end{enumerate} 